examples/riscv/incr/incr_propScript.sml
@@ -57,6 +57,14 @@ Proof
  ACCEPT_TAC bir_cont_incr_thm
 QED
 
+(* --------------------- *)
+(* Auxiliary definitions *)
+(* --------------------- *)
+
+val progbin_tm = (fst o dest_eq o concl) bir_incr_progbin_def;
+val riscv_pre_tm = (fst o dest_comb o lhs o snd o strip_forall o concl) riscv_incr_pre_def;
+val riscv_post_tm = (fst o dest_comb o lhs o snd o strip_forall o concl) riscv_incr_post_def;
+
 (* ---------------------------------- *)
 (* Backlifting BIR contract to RISC-V *)
 (* ---------------------------------- *)
@@ -64,8 +72,8 @@ QED
 val riscv_cont_incr_thm =
  get_riscv_contract_sing
   bir_cont_incr
-  ``bir_incr_progbin``
-  ``riscv_incr_pre pre_x10`` ``riscv_incr_post pre_x10`` bir_incr_prog_def
+  progbin_tm
+  riscv_pre_tm riscv_post_tm bir_incr_prog_def
   [bir_incr_pre_def]
   bir_incr_pre_def incr_riscv_pre_imp_bir_pre_thm
   [bir_incr_post_def] incr_riscv_post_imp_bir_post_thm
