examples/riscv/incr/incr_symb_transfScript.sml
@@ -19,8 +19,8 @@ val _ = new_theory "incr_symb_transf";
 val init_addr_tm = (snd o dest_eq o concl) incr_init_addr_def;
 val end_addr_tm = (snd o dest_eq o concl) incr_end_addr_def;
 
-val bspec_pre_tm = ``bspec_incr_pre pre_x10``;
-val bspec_post_tm = ``bspec_incr_post pre_x10``;
+val bspec_pre_tm = (lhs o snd o strip_forall o concl) bspec_incr_pre_def;
+val bspec_post_tm = (lhs o snd o strip_forall o concl) bspec_incr_post_def;
 
 (* ------------------------------- *)
 (* BIR symbolic execution analysis *)
@@ -28,7 +28,8 @@ val bspec_post_tm = ``bspec_incr_post pre_x10``;
 
 val bspec_cont_thm =
  bir_symb_transfer init_addr_tm end_addr_tm bspec_pre_tm bspec_post_tm
-  bir_incr_prog_def incr_birenvtyl_def bspec_incr_pre_def bspec_incr_post_def incr_prog_vars_def
+  bir_incr_prog_def incr_birenvtyl_def
+  bspec_incr_pre_def bspec_incr_post_def incr_prog_vars_def
   incr_symb_analysis_thm incr_bsysprecond_thm incr_prog_vars_thm;
 
 Theorem bspec_cont_incr:
